Challenge/Ripemd160/Submission/Proofs/Bytecode/GuardInstructionWindow.lean
@@ -66,7 +66,7 @@ def tail : List Instr :=
   op 0x36,
   op 0x8c,
   op 0x14,
-  .push 2 4740,
+  .push 2 4726,
   op 0x57,
   op 0x50,
   op 0x50,
@@ -87,14 +87,14 @@ def tail : List Instr :=
   .push 1 32,
   op 0x1b,
   op 0x17,
-  .push 2 257,
-  op 0x84,
-  op 0x82,
-  op 0x83,
+  op 0x80,
+  op 0x80,
   .push 1 8,
   op 0x1c,
   op 0x18,
+  op 0x84,
   op 0x16,
+  .push 2 257,
   op 0x02,
   op 0x18,
   op 0x80,
@@ -135,7 +135,7 @@ def tail : List Instr :=
   op 0x1c,
   op 0x90,
   op 0x81,
-  .push 2 4717,
+  .push 2 4703,
   op 0x57,
   op 0x50,
   op 0x50,
@@ -146,7 +146,6 @@ def tail : List Instr :=
   op 0x36,
   .push 0 0,
   op 0x37,
-  .push 1 128,
   op 0x36,
   .push 1 3,
   op 0x1b,
@@ -158,19 +157,17 @@ def tail : List Instr :=
   op 0x52,
   .push 1 144,
   op 0x52,
-  op 0x80,
+  .push 1 128,
   .push 2 522,
   op 0x52,
-  op 0x80,
+  .push 19 2854495385411919762116571938898990272765493376,
   .push 1 54,
-  op 0x52,
-  .push 1 36,
   op 0x52,
   op 0x36,
   .push 1 29,
   op 0x1c,
   op 0x15,
-  .push 2 904,
+  .push 2 902,
   op 0x57,
   op 0x36,
   .push 1 29,
@@ -189,7 +186,7 @@ def tail : List Instr :=
   op 0x52,
   .push 2 270,
   op 0x52,
-  .push 2 904,
+  .push 2 902,
   op 0x56,
   op 0x5b,
   .push 17 342276208914615837337402008677671501826,
@@ -233,19 +230,19 @@ def tail : List Instr :=
   .push 0 0,
   op 0xf3
 ]
-theorem tail_eq : Artifact.submissionArtifact.instructions.drop 3577 = tail := by rfl
+theorem tail_eq : Artifact.submissionArtifact.instructions.drop 3579 = tail := by rfl
 
-theorem pc_base : Artifact.submissionArtifact.instructionPC 3577 = 4573 := by
+theorem pc_base : Artifact.submissionArtifact.instructionPC 3579 = 4559 := by
   rw [instructionPC_eq_byteLength]
   rfl
 
 theorem get (index : Nat) :
-    Artifact.submissionArtifact.instructions[3577 + index]? = tail[index]? := by
+    Artifact.submissionArtifact.instructions[3579 + index]? = tail[index]? := by
   rw [← InstructionWindow.get_drop, tail_eq]
 
 theorem pc (index : Nat) :
-    Artifact.submissionArtifact.instructionPC (3577 + index) =
-      4573 + byteLength (tail.take index) := by
+    Artifact.submissionArtifact.instructionPC (3579 + index) =
+      4559 + byteLength (tail.take index) := by
   rw [InstructionWindow.pc_drop, pc_base, tail_eq]
 
 #print axioms get
